[SI_new_model] got fixed the RA which is set to (authR (gmapUR nat (agreeR ((gmapUR Key ((max_prefix_listR write_eventO))))))). Fixed definitionsso now proofs remain to be fixed.

aneris/examples/snapshot_isolation/proof/resources/server_resources.v
@@ -57,174 +57,75 @@ Section ConnectedClients.
 
 End ConnectedClients.
 
-(*----------------------------------------------------------------------------*)
-(** Resources embedding the model of the global memory and snapshots.         *)
-(*----------------------------------------------------------------------------*)
-
 (*---------------------------------------------------------------------------*)
 (** ----------------------- Resources for Snapshots ------------------------ *)
 (*---------------------------------------------------------------------------*)
 Section Snapshot_Resources.
   Context `{!anerisG Mdl Σ, !User_params, !IDBG Σ}.
   Context (γTrns : gname).
-
-  (** Snapshots related to a transaction identified by a ghost name γt. *)
-  Section Snapshot_at_given_gname.
-    Context (γt : gname).
-    
-    Definition ownSnapFragGname (k : Key) (h : whist) : iProp Σ :=
-      own γt (◯ {[ k := to_max_prefix_list h]}).
-
-    Lemma ownSnapFragGnamePersistent k h:
-      Persistent (ownSnapFragGname k h).
-    Proof. apply _. Qed.
   
-    Definition global_memUR M : gmapUR Key (max_prefix_listR write_eventO) :=
-      (to_max_prefix_list <$> M :
-        gmapUR Key (max_prefix_listR write_eventO)).
+  Definition global_memUR M : gmapUR Key (max_prefix_listR write_eventO) :=
+    (to_max_prefix_list <$> M :
+      gmapUR Key (max_prefix_listR write_eventO)).
 
-    Definition ownSnapFragMemGname M : iProp Σ :=
-      own γt (◯ global_memUR M).
+  Definition ownSnapFrag (t : nat)  (M : gmap Key (list write_eventO)) : iProp Σ :=
+    own γTrns (◯ {[ t := to_agree (global_memUR M) ]}).
 
-    Lemma ownSnapFragMemGnamePersistent M:
-      Persistent (ownSnapFragMemGname M).
-    Proof. apply _. Qed.
-    
-    Definition ownSnapAuthGname (M : global_mem) : iProp Σ :=
-      own γt (● global_memUR M).
-
-    Lemma ownSnapFragGname_lookup M k h :
-      ownSnapAuthGname M ⊢
-      ownSnapFragGname k h -∗
-      ∃ h', ⌜h `prefix_of` h' ∧ M !! k = Some h'⌝.
-    Proof.
-      iIntros "H1 H2".
-      iDestruct (own_valid_2 with "H1 H2")
-        as %[Hv1 Hv2]%auth_both_valid_discrete.
-      rewrite singleton_included_l in Hv1.
-      destruct Hv1 as (y & Hvy & Hv1).
-      rewrite Some_included_total in Hv1.
-      rewrite lookup_fmap in Hvy.
-      destruct (M !! k) eqn:Heq; rewrite Heq in Hvy;
-        simplify_eq /=; [| by inversion Hvy].
-      apply Some_equiv_inj in Hvy.
-      rewrite -Hvy to_max_prefix_list_included in Hv1.
-      destruct Hv1 as (l0 & Hl0).
-      fold_leibniz.
-      iPureIntro; exists l. split; last done.
-      by rewrite Hl0; apply prefix_app_r.
-    Qed.
-
-    (* We do not need this lemma actually *)
-    (* Lemma ownSnapFragGname_prefix k h h':
-      ownSnapFragGname k h ⊢ ownSnapFragGname k h' -∗
-        ⌜h `prefix_of` h' ∨ h' `prefix_of` h⌝.
-    Proof.
-      iIntros "Hobs1 Hobs2".
-      iDestruct (own_valid_2 with "Hobs1 Hobs2") as %Hvalid.
-      rewrite auth_frag_op_valid singleton_op singleton_valid
-        in Hvalid.
-      by rewrite to_max_prefix_list_op_valid_L in Hvalid.
-    Qed. *)
-
-    Lemma get_ownSnapFragGname_prefix M k h hl:
-      M !! k = Some h →
-      hl `prefix_of` h →
-      ownSnapAuthGname M ⊢
-        |==> ownSnapAuthGname M ∗ ownSnapFragGname k hl.
-    Proof.
-      iIntros (HMk h_hl) "?".
-      iApply own_op.
-      iApply own_update; last done.
-      apply auth_update_dfrac_alloc.
-      {
-        apply gmap_core_id=>i x/lookup_singleton_Some[_<-].
-        apply max_prefix_list.mono_list_lb_core_id.
-      }
-      apply (@singleton_included_l _ _ _ (max_prefix_listR write_eventO)).
-      exists (to_max_prefix_list h).
-      split; first by rewrite lookup_fmap HMk.
-      apply Some_included_2.
-      apply (@to_max_prefix_list_included_L write_eventO); last done.
-      apply _.
-    Qed.
+  Lemma ownSnapFragPersistent t M:
+    Persistent (ownSnapFrag t M).
+  Proof. apply _. Qed.
   
-  Lemma get_ownSnapFragGname M k h :
-      M !! k = Some h →
-      ownSnapAuthGname M ⊢ |==> ownSnapAuthGname M ∗ ownSnapFragGname k h.
+  Definition ownSnapAuth (S : gmap nat global_mem) : iProp Σ :=
+    own γTrns (● (((λ M, to_agree (global_memUR M)) <$> S) : gmap _ _)).
+
+   Lemma ownSnapAgree t M S :
+    ownSnapFrag t M -∗
+    ownSnapAuth S -∗
+      ⌜S !! t = Some M⌝. 
   Proof.
-    intro HMk.
-    by iApply get_ownSnapFragGname_prefix.
+    iIntros "Hf Ha".
+    iDestruct (own_valid_2 with "Ha Hf")
+      as %[Hv1 Hv2]%auth_both_valid_discrete.
+    rewrite singleton_included_l in Hv1.
+    destruct Hv1 as (y & Hvy & Hv1).
+    rewrite Some_included_total in Hv1.
+    rewrite lookup_fmap in Hvy.
+    destruct (S !! t) eqn:HSt; last first. rewrite HSt in Hvy.  inversion Hvy.
+    rewrite HSt in Hvy. 
+    simplify_eq/=. iPureIntro. inversion Hvy. rewrite -H2 in Hv1.
+    apply to_agree_included in Hv1. apply leibniz_equiv. symmetry.
+    simplify_eq /=. f_equal. f_equal. rewrite /global_memUR in Hv1. 
+    apply Some_equiv_eq. exists M. split; first done.
+    apply (map_fmap_equiv_inj to_max_prefix_list) in Hv1; first done.
+    apply _. 
   Qed.
   
-  End Snapshot_at_given_gname.
-
-  Section Snapshots.
+  Lemma ownSnapFragAgree t M1 M2 :
+    ownSnapFrag t M1 -∗
+    ownSnapFrag t M2 -∗
+      ⌜M1 = M2⌝. 
+  Proof.
+    iIntros "Hf1 Hf2".
+    rewrite /ownSnapFrag.
+    iDestruct (own_valid_2 with "Hf1 Hf2") as %Hval.
+    rewrite -auth_frag_op singleton_op  in Hval.
+    apply auth_frag_valid_1 in Hval.
+    specialize (Hval t).
+    rewrite lookup_singleton in Hval.
+    rewrite Some_op in Hval.
+    iPureIntro.
+    revert Hval.
+    rewrite Some_valid.
+    intros Hval.
+    eapply (to_agree_op_inv (A:= _ )) in Hval.
+    apply leibniz_equiv.
+    rewrite /global_memUR in Hval.
+    eapply (map_fmap_equiv_inj to_max_prefix_list) in Hval; first done.
+    apply _.
+  Qed.
     
-    (** A transaction identified by the start time ts and a ghost name γTr. *)
-    Definition ownTrnFrag (t : nat) (γt : gname) : iProp Σ :=
-      own γTrns (◯ {[ t := to_agree γt ]}).
-
-    Definition ownSnapshotsNamesAuth (S : gmap nat gname) : iProp Σ :=
-      own γTrns (● (to_agree <$> S : gmap _ _)).
-
-    Definition ownSnapFrag γt (t : nat) (k : Key) (h : whist) : iProp Σ :=
-      ownTrnFrag t γt ∗ ownSnapFragGname γt k h .
-
-    Lemma ownSnapFragPersistent γt t k h :
-      Persistent (ownSnapFrag γt t k h).
-    Proof. apply _. Qed.
-
-    (** Importantly, note that there is currently no relation between snapshots
-        for two given transactions. We only relate snapshots to the state of 
-        the global memory. *)
-    Definition ownSnapshotsAuth (Sγ : gmap nat gname) (S : snapshots) : iProp Σ :=
-      ownSnapshotsNamesAuth Sγ ∗
-      ([∗ map] t ↦ γt ; Mt ∈ Sγ ; S, ownTrnFrag t γt ∗ ownSnapAuthGname γt Mt).
-
-    Lemma ownSnapFrag_lookup Sγ S M γ t k h :
-      ownSnapshotsAuth Sγ S ⊢
-      ⌜Sγ !! t = Some γ⌝ -∗
-      ⌜S !! t = Some M⌝ -∗
-      ownSnapFrag γ t k h -∗
-      ∃ h', ⌜h `prefix_of` h' ∧ M !! k = Some h'⌝.
-    Proof.
-      iIntros "(HAuthNames & HAuth) %Hγ %HM #(Hf1 & Hf2)".
-      iDestruct (big_sepM2_lookup with "[$HAuth]") as "(_ & HauthM)"; try eauto.
-      iApply (ownSnapFragGname_lookup with "[$HauthM][$Hf2]").
-    Qed.
-
-    Lemma get_ownSnapFrag_prefix Sγ S M k h hl t γ:
-      Sγ !! t = Some γ →
-      S !! t = Some M →
-      M !! k = Some h →
-      hl `prefix_of` h →
-      ownSnapshotsAuth Sγ S ⊢
-      |==> ownSnapshotsAuth Sγ S ∗ ownSnapFrag γ t k hl.
-    Proof.
-      iIntros (Hsg HS HM Hpre) "(Htrs & Hauth)".
-      iDestruct (big_sepM2_lookup_acc with "[$Hauth]")
-        as "((#Ht & Ha) & Hacc)"; try eauto.
-      iMod (get_ownSnapFragGname_prefix γ M k h hl HM Hpre with "[Ha]")
-        as "(Ha & Hf)"; try eauto.
-      iFrame "#∗".
-      iApply "Hacc".
-      by iFrame "#∗".
-    Qed.
-    
-    Lemma get_ownSnapFrag Sγ S M t k h γ :
-      Sγ !! t = Some γ →
-      S !! t = Some M →
-      M !! k = Some h →
-      ownSnapshotsAuth Sγ S ⊢ |==>  ownSnapshotsAuth Sγ S ∗ ownSnapFrag γ t k h.
-    Proof.
-      iIntros (???) "Ha".
-      by iApply (get_ownSnapFrag_prefix with "[$Ha]").
-    Qed.
-
-  End Snapshots.
-
 End Snapshot_Resources.
+   
 
 (*---------------------------------------------------------------------------*)
 (** ------------------- Resources for Global State ------------------------- *)
